Dafny/LLVM/generalInstructions.i.dfy
@@ -88,6 +88,7 @@ lemma lvm_lemma_Add(lvm_b0:lvm_codes, lvm_s0:lvm_state, lvm_sN:lvm_state,
     assert ValidState(lvm_sM);
     assert ValidOperand(lvm_sM,dst);
     assert evalIns(lvm_code_Add(dst, size,src1,src2).ins,lvm_s0,lvm_sM);
+    assert NextStep(lvm_s0,lvm_sM,evalInsStep(lvm_code_Add(dst, size,src1,src2).ins));
     // var evalA := evalADD(OperandContents(lvm_s0,dst).itype.size,OperandContents(lvm_s0,src1),OperandContents(lvm_s0,src2));
     // assert evalUpdate(lvm_s0, dst, evalA,lvm_sM);
     assert (forall d :: ValidOperand(lvm_s0,d) && d != dst ==> ValidOperand(lvm_sM,d) && OperandContents(lvm_s0,d) == OperandContents(lvm_sM,d));
@@ -145,6 +146,8 @@ ensures lvm_s0.m == lvm_sM.m;
 
   assert ValidState(lvm_sM);
   assert evalCode_lax(lvm_cM, lvm_s0, lvm_sM);
+  assert NextStep(lvm_s0,lvm_sM,evalInsStep(lvm_code_GetElementPtr(dst,t,op1,op2).ins));
+
 }
 
 
@@ -173,7 +176,7 @@ lemma lvm_lemma_Ret(lvm_b0:lvm_codes, lvm_s0:lvm_state, lvm_sN:lvm_state,dst:lvm
   ensures  lvm_state_eq(lvm_sM,  lvm_s0)
   ensures lvm_bM == lvm_b0.tl;
   ensures forall d :: ValidOperand(lvm_s0,d) && d != dst ==> ValidOperand(lvm_sM,d) && OperandContents(lvm_s0,d) == OperandContents(lvm_sM,d)
-  ensures StateNext(lvm_s0,lvm_sM)
+  ensures StateNext(lvm_s0,lvm_sM);
 
 {
   
@@ -189,6 +192,8 @@ lemma lvm_lemma_Ret(lvm_b0:lvm_codes, lvm_s0:lvm_state, lvm_sN:lvm_state,dst:lvm
 
   assert ValidState(lvm_sM);
   assert evalCode(lvm_cM, lvm_s0, lvm_sM);
+  assert NextStep(lvm_s0,lvm_sM,evalInsStep(lvm_code_Ret(op1).ins));
+
 }
 
 
@@ -265,6 +270,8 @@ lemma lvm_lemma_Load(lvm_b0:lvm_codes, lvm_s0:lvm_state, lvm_sN:lvm_state,dst:lv
   
   assert lvm_sM.ok ==> ValidState(lvm_sM);
   assert lvm_sM.ok ==> evalCode_lax(lvm_cM, lvm_s0, lvm_sM);
+  assert NextStep(lvm_s0,lvm_sM,evalInsStep(lvm_LOAD(dst,lvm_s0.m,t,op1).ins));
+
 }
 
 
@@ -323,6 +330,7 @@ lemma lvm_lemma_Zext(lvm_b0:lvm_codes, lvm_s0:lvm_state, lvm_sN:lvm_state,
 
   assert ValidState(lvm_sM);
   assert evalCode_lax(lvm_cM, lvm_s0, lvm_sM);
+  assert NextStep(lvm_s0,lvm_sM,evalInsStep(lvm_code_ZEXT(dst,t,op1,dstSize).ins));
 }
 
 
@@ -381,6 +389,8 @@ lemma lvm_lemma_Sext(lvm_b0:lvm_codes, lvm_s0:lvm_state, lvm_sN:lvm_state,
 
     assert ValidState(lvm_sM);
     assert evalCode_lax(lvm_cM, lvm_s0, lvm_sM);
+    assert NextStep(lvm_s0,lvm_sM,evalInsStep(lvm_code_SEXT(dst,t,op1,dstSize).ins));
+
 }
 
 function method lvm_code_SHL(dst:lvm_operand_opr,src:lvm_operand_opr,shiftAmt:lvm_operand_opr):(out:lvm_code)
@@ -443,6 +453,8 @@ lemma lvm_lemma_Shl(lvm_b0:lvm_codes, lvm_s0:lvm_state, lvm_sN:lvm_state,
 
     assert ValidState(lvm_sM);
     assert evalCode_lax(lvm_cM, lvm_s0, lvm_sM);
+    assert NextStep(lvm_s0,lvm_sM,evalInsStep(lvm_code_SHL(dst,src,shiftAmt).ins));
+
 }
 
 function method lvm_code_ICMP(dst:lvm_operand_opr,cond:lvm_cond,size:nat,op1:lvm_operand_opr,op2:lvm_operand_opr):(out:lvm_code)
@@ -499,6 +511,8 @@ lemma lvm_lemma_Icmp(lvm_b0:lvm_codes, lvm_s0:lvm_state, lvm_sN:lvm_state,
 
     assert ValidState(lvm_sM);
     assert evalCode_lax(lvm_cM, lvm_s0, lvm_sM);
+    assert NextStep(lvm_s0,lvm_sM,evalInsStep(lvm_code_ICMP(dst,cond,size,op1,op2).ins));
+
 
 }
 
@@ -543,6 +557,8 @@ lemma lvm_lemma_Empty(lvm_b0:lvm_codes, lvm_s0:lvm_state, lvm_sN:lvm_state)
     lvm_sM := lvm_lemma_empty(lvm_s0, lvm_sM);
     assert ValidState(lvm_sM);
     assert lvm_s0 == lvm_sM;
+    assert NextStep(lvm_s0,lvm_sM,stutterStep());
+
 }
 
 
