Dafny/examples/Challenge5.i.dfy
@@ -1,0 +1,352 @@
+include "../LLVM/llvm.i.dfy"
+include "../LLVM/control_flow.i.dfy"
+include "../LLVM/generalInstructions.i.dfy"
+include "../LLVM/types.dfy"
+include "../LLVM/memory.i.dfy"
+include "../LLVM/Operations/otherOperations.i.dfy"
+
+
+module challenge5 {
+    import opened LLVM_def
+    import opened control_flow
+    import opened general_instructions
+    import opened types
+    import opened memory
+    import opened other_operations_i
+// **** MAIN.C MAIN WHILE LOOP ****
+
+// do.body:                                          ; preds = %schedule_timer.exit, %cleanup
+//   %report_timer.0295 = phi i64 [ %report_timer.2, %cleanup ], [ %call44, %schedule_timer.exit ]
+//   %84 = call { i64, i64* } asm sideeffect "cld; rep; stosq", "={cx},={di},{ax},0,1,~{memory},~{dirflag},~{fpsr},~{flags}"(i32 0, i64 16, i64* nonnull %arrayidx47) #24, !srcloc !35
+//   %85 = load i64, i64* %arrayidx51, align 8, !tbaa !36
+//   %or = or i64 %85, %shl
+//   store i64 %or, i64* %arrayidx51, align 8, !tbaa !36
+//   store <2 x i64> <i64 0, i64 50>, <2 x i64>* %timeout, align 16, !tbaa !36
+//   %call52 = call i32 @select(i32 %add, %struct.__sigset_t* nonnull %readfds, %struct.__sigset_t* null, %struct.__sigset_t* null, %struct.timeval* nonnull %tmpcast303) #24
+//   %cmp53 = icmp sgt i32 %call52, 0
+//   br i1 %cmp53, label %if.then55, label %if.end86
+
+// if.then55:                                        ; preds = %do.body
+//   %call56 = call i64 @read(i32 %call8, i8* nonnull %80, i64 16) #24
+//   %cmp57 = icmp slt i64 %call56, 0
+//   br i1 %cmp57, label %cleanup.thread, label %if.end60
+
+// cleanup.thread:                                   ; preds = %if.then55
+//   call void @perror(i8* getelementptr inbounds ([9 x i8], [9 x i8]* @.str.8, i64 0, i64 0)) #23
+//   br label %cleanup176
+
+// if.end60:                                         ; preds = %if.then55
+//   %86 = load i64, i64* %81, align 8
+//   %87 = load i64, i64* %82, align 8
+//   call void @logging_handler(i64 %86, i64 %87) #24
+//   %88 = trunc i64 %86 to i32
+//   %and61 = and i32 %88, 536870911
+//   store i32 %and61, i32* %can_id, align 8, !tbaa !37
+//   %89 = and i32 %88, 15728640
+//   %cmp.i261 = icmp eq i32 %89, 15728640
+//   %and6.i = lshr i32 %88, 8
+//   %shr7.i = and i32 %and6.i, 262143
+//   %and3.i = lshr i32 %and61, 8
+//   %shr10.i = and i32 %and3.i, 261888
+//   %storemerge.i = select i1 %cmp.i261, i32 %shr7.i, i32 %shr10.i
+//   %90 = lshr i64 %87, 16
+//   %91 = trunc i64 %90 to i32
+//   switch i32 %storemerge.i, label %if.end86 [
+//     i32 65265, label %if.then65
+//     i32 64972, label %if.then68
+//     i32 60928, label %if.then74
+//     i32 59904, label %if.then80
+//   ]
+
+// if.then65:                                        ; preds = %if.end60
+//   %92 = and i64 %87, 51539607552
+//   %tobool.not.i = icmp ne i64 %92, 0
+//   %conv8.i263 = zext i1 %tobool.not.i to i8
+//   store i8 %conv8.i263, i8* %brake_state.i, align 1, !tbaa !38
+//   br i1 %tobool.not.i, label %if.then.i265, label %if.else.i266
+
+// if.then.i265:                                     ; preds = %if.then65
+//   %93 = lshr i64 %87, 16
+//   %94 = trunc i64 %93 to i32
+//   %shl.i = and i32 %94, 65280
+//   %conv2.i = and i32 %91, 255
+//   %add.i = or i32 %shl.i, %conv2.i
+//   %cmp.not.i = icmp eq i32 %add.i, 0
+//   br i1 %cmp.not.i, label %if.end86, label %land.lhs.true.i
+
+// land.lhs.true.i:                                  ; preds = %if.then.i265
+//   %95 = load i8, i8* %has_flashed17.i, align 4, !tbaa !40
+//   %tobool14.not.i = icmp eq i8 %95, 0
+//   br i1 %tobool14.not.i, label %if.then15.i, label %if.end86
+
+// if.then15.i:                                      ; preds = %land.lhs.true.i
+//   store i8 1, i8* %flash_lock16.i, align 2, !tbaa !41
+//   br label %if.end86
+
+// if.else.i266:                                     ; preds = %if.then65
+//   store i8 0, i8* %flash_lock16.i, align 2, !tbaa !41
+//   store i8 0, i8* %has_flashed17.i, align 4, !tbaa !40
+//   br label %if.end86
+
+// if.then68:                                        ; preds = %if.end60
+//   %96 = lshr i64 %87, 12
+//   %97 = trunc i64 %96 to i8
+//   %98 = and i8 %97, 15
+//   store i8 %98, i8* %signal.i, align 1, !tbaa !42
+//   br label %if.end86
+
+// if.then74:                                        ; preds = %if.end60
+//   %conv12.i = trunc i64 %86 to i8
+//   call void @rx_claim_routine(i8 zeroext %conv12.i, i8* nonnull %arraydecay76, i32 %call8, i32* %11)
+//   br label %if.end86
+
+// if.then80:                                        ; preds = %if.end60
+//   %99 = and i32 %and3.i, 255
+//   %conv81 = select i1 %cmp.i261, i32 255, i32 %99
+//   %100 = load i8, i8* getelementptr inbounds (%struct.conf_t, %struct.conf_t* @conf, i64 0, i32 3), align 8, !tbaa !28
+//   %conv.i268 = zext i8 %100 to i32
+//   %cmp.i269 = icmp eq i32 %conv81, %conv.i268
+//   %cmp2.i = icmp eq i32 %conv81, 255
+//   %or.cond.i = or i1 %cmp2.i, %cmp.i269
+//   br i1 %or.cond.i, label %if.then.i271, label %if.end86
+
+// if.then.i271:                                     ; preds = %if.then80
+//   %call.i270 = call i64 @write(i32 %call8, i8* bitcast (%struct.can_frame* getelementptr inbounds (%struct.conf_t, %struct.conf_t* @conf, i64 0, i32 7) to i8*), i64 16) #24
+//   %cmp4.not.i = icmp eq i64 %call.i270, 16
+//   br i1 %cmp4.not.i, label %if.end86, label %if.then6.i
+
+// if.then6.i:                                       ; preds = %if.then.i271
+//   call void (i32, i8*, ...) @err(i32 1, i8* getelementptr inbounds ([33 x i8], [33 x i8]* @.str.14, i64 0, i64 0)) #25
+//   unreachable
+
+// if.end86:                                         ; preds = %if.then74, %if.then68, %if.end60, %if.then.i265, %land.lhs.true.i, %if.then15.i, %if.else.i266, %if.then80, %if.then.i271, %do.body
+//   call void @turn_signal_routine(%struct.Bumper* %10) #24
+//   call void @brake_routine(%struct.Bumper* %10) #24
+//   %101 = load i8, i8* %outer_left, align 16, !tbaa !43
+//   %102 = load i8, i8* %inner_left, align 1, !tbaa !44
+//   %103 = load i8, i8* %inner_right, align 2, !tbaa !45
+//   %104 = load i8, i8* %outer_right, align 1, !tbaa !46
+//   %tobool88.not = icmp eq i8 %101, 0
+//   %cond = select i1 %tobool88.not, i32 10, i32 100
+//   call void @set_duty(i32 1, i32 %cond) #24
+//   %tobool90.not = icmp eq i8 %102, 0
+//   %cond91 = select i1 %tobool90.not, i32 10, i32 100
+//   call void @set_duty(i32 2, i32 %cond91) #24
+//   %tobool93.not = icmp eq i8 %103, 0
+//   %cond94 = select i1 %tobool93.not, i32 10, i32 100
+//   call void @set_duty(i32 3, i32 %cond94) #24
+//   %tobool96.not = icmp eq i8 %104, 0
+//   %cond97 = select i1 %tobool96.not, i32 10, i32 100
+//   call void @set_duty(i32 4, i32 %cond97) #24
+//   %cond100 = select i1 %tobool88.not, i8* getelementptr inbounds ([2 x i8], [2 x i8]* @.str.11, i64 0, i64 0), i8* getelementptr inbounds ([2 x i8], [2 x i8]* @.str.10, i64 0, i64 0)
+//   %cond103 = select i1 %tobool90.not, i8* getelementptr inbounds ([2 x i8], [2 x i8]* @.str.11, i64 0, i64 0), i8* getelementptr inbounds ([2 x i8], [2 x i8]* @.str.10, i64 0, i64 0)
+//   %cond106 = select i1 %tobool93.not, i8* getelementptr inbounds ([2 x i8], [2 x i8]* @.str.11, i64 0, i64 0), i8* getelementptr inbounds ([2 x i8], [2 x i8]* @.str.10, i64 0, i64 0)
+//   %cond109 = select i1 %tobool96.not, i8* getelementptr inbounds ([2 x i8], [2 x i8]* @.str.11, i64 0, i64 0), i8* getelementptr inbounds ([2 x i8], [2 x i8]* @.str.10, i64 0, i64 0)
+//   %105 = load i32, i32* getelementptr inbounds (%struct.conf_t, %struct.conf_t* @conf, i64 0, i32 6), align 4, !tbaa !47
+//   %106 = load i8, i8* getelementptr inbounds (%struct.conf_t, %struct.conf_t* @conf, i64 0, i32 3), align 8, !tbaa !28
+//   %conv110 = zext i8 %106 to i32
+//   %call111 = call i32 (i8*, ...) @printf(i8* nonnull dereferenceable(1) getelementptr inbounds ([50 x i8], [50 x i8]* @.str.9, i64 0, i64 0), i8* %cond100, i8* %cond103, i8* %cond106, i8* %cond109, i32 %105, i32 %conv110)
+//   %107 = load i32, i32* getelementptr inbounds (%struct.conf_t, %struct.conf_t* @conf, i64 0, i32 6), align 4, !tbaa !47
+//   switch i32 %107, label %cleanup [
+//     i32 1, label %if.then114
+//     i32 2, label %if.then121
+//   ]
+
+// if.then114:                                       ; preds = %if.end86
+//   %108 = load i32, i32* getelementptr inbounds (%struct.conf_t, %struct.conf_t* @conf, i64 0, i32 5), align 8, !tbaa !32
+//   %tobool115.not = icmp eq i32 %108, 0
+//   br i1 %tobool115.not, label %cleanup, label %if.then116
+
+// if.then116:                                       ; preds = %if.then114
+//   store i32 2, i32* getelementptr inbounds (%struct.conf_t, %struct.conf_t* @conf, i64 0, i32 6), align 4, !tbaa !47
+//   br label %cleanup
+
+// if.then121:                                       ; preds = %if.end86
+//   store i8 0, i8* %arraydecay76, align 8, !tbaa !10
+//   %not.tobool88.not = xor i1 %tobool88.not, true
+//   %conv127 = sext i1 %not.tobool88.not to i8
+//   store i8 %conv127, i8* %arrayidx129, align 1, !tbaa !10
+//   store i8 0, i8* %arrayidx131, align 2, !tbaa !10
+//   %not.tobool90.not = xor i1 %tobool90.not, true
+//   %conv135 = sext i1 %not.tobool90.not to i8
+//   store i8 %conv135, i8* %arrayidx137, align 1, !tbaa !10
+//   store i8 0, i8* %arrayidx139, align 4, !tbaa !10
+//   %not.tobool93.not = xor i1 %tobool93.not, true
+//   %conv143 = sext i1 %not.tobool93.not to i8
+//   store i8 %conv143, i8* %arrayidx145, align 1, !tbaa !10
+//   store i8 0, i8* %arrayidx147, align 2, !tbaa !10
+//   %not.tobool96.not = xor i1 %tobool96.not, true
+//   %conv151 = sext i1 %not.tobool96.not to i8
+//   store i8 %conv151, i8* %arrayidx153, align 1, !tbaa !10
+//   %109 = load i8, i8* getelementptr inbounds (%struct.conf_t, %struct.conf_t* @conf, i64 0, i32 3), align 8, !tbaa !28
+//   %conv154 = zext i8 %109 to i32
+//   %or157 = or i32 %conv154, -1661059072
+//   store i32 %or157, i32* %can_id, align 8, !tbaa !37
+//   store i8 8, i8* %can_dlc, align 4, !tbaa !48
+//   %call159 = call i64 @clock() #24
+//   %sub = sub nsw i64 %call159, %report_timer.0295
+//   %cmp161 = icmp sgt i64 %sub, 100000
+//   br i1 %cmp161, label %if.then163, label %cleanup
+
+// if.then163:                                       ; preds = %if.then121
+//   %call164 = call i64 @write(i32 %call8, i8* nonnull %80, i64 16) #24
+//   %cmp165.not = icmp eq i64 %call164, 16
+//   br i1 %cmp165.not, label %if.end168, label %if.then167
+
+// if.then167:                                       ; preds = %if.then163
+//   call void (i32, i8*, ...) @err(i32 1, i8* getelementptr inbounds ([31 x i8], [31 x i8]* @.str.7.12, i64 0, i64 0)) #25
+//   unreachable
+
+// if.end168:                                        ; preds = %if.then163
+//   %call169 = call i64 @clock() #24
+//   br label %cleanup
+
+// cleanup:                                          ; preds = %if.then116, %if.then114, %if.then121, %if.end168, %if.end86
+//   %report_timer.2 = phi i64 [ %report_timer.0295, %if.then116 ], [ %report_timer.0295, %if.then114 ], [ %call169, %if.end168 ], [ %report_timer.0295, %if.then121 ], [ %report_timer.0295, %if.end86 ]
+//   %110 = load i32, i32* getelementptr inbounds (%struct.conf_t, %struct.conf_t* @conf, i64 0, i32 4), align 4, !tbaa !34
+//   %tobool.not = icmp eq i32 %110, 0
+//   br i1 %tobool.not, label %do.body, label %while.end174, !llvm.loop !49
+
+// **** END MAIN FOR LOOP ****
+
+// **** LOGGING.C WRITE_ENCRYPTED() ****
+
+// ; Function Attrs: nounwind uwtable
+// define dso_local void @write_encrypted() local_unnamed_addr #5 {
+// entry:
+//   %bytes_written = alloca i32, align 4
+//   %0 = bitcast i32* %bytes_written to i8*
+//   call void @llvm.lifetime.start.p0i8(i64 4, i8* nonnull %0) #24
+//   %call = tail call noalias align 16 dereferenceable_or_null(112) i8* @malloc(i64 112) #24
+//   tail call void @llvm.memcpy.p0i8.p0i8.i64(i8* noundef nonnull align 16 dereferenceable(112) %call, i8* noundef nonnull align 8 dereferenceable(112) getelementptr inbounds (%struct.MBlock, %struct.MBlock* @mblock, i64 0, i32 0, i64 0), i64 112, i1 false)
+//   %call1 = tail call noalias align 16 dereferenceable_or_null(120) i8* @malloc(i64 120) #24
+//   %call2 = tail call i32 @encrypt(i8* %call, i32 112, i8* getelementptr inbounds ([32 x i8], [32 x i8]* @KEY, i64 0, i64 0), i8* getelementptr inbounds ([16 x i8], [16 x i8]* @IV, i64 0, i64 0), i8* %call1) #24
+//   store i32 %call2, i32* %bytes_written, align 4, !tbaa !3
+//   %1 = load %struct._IO_FILE*, %struct._IO_FILE** @wfd, align 8, !tbaa !14
+//   %call3 = call i64 @fwrite(i8* nonnull %0, i64 4, i64 1, %struct._IO_FILE* %1)
+//   %cmp = icmp eq i64 %call3, 0
+//   br i1 %cmp, label %if.then, label %if.end
+
+// if.then:                                          ; preds = %entry
+//   tail call void @perror(i8* getelementptr inbounds ([27 x i8], [27 x i8]* @.str.4, i64 0, i64 0)) #23
+//   br label %if.end
+
+// if.end:                                           ; preds = %if.then, %entry
+//   %2 = load i32, i32* %bytes_written, align 4, !tbaa !3
+//   %conv = sext i32 %2 to i64
+//   %3 = load %struct._IO_FILE*, %struct._IO_FILE** @wfd, align 8, !tbaa !14
+//   %call4 = tail call i64 @fwrite(i8* %call1, i64 1, i64 %conv, %struct._IO_FILE* %3)
+//   %cmp5 = icmp eq i64 %call4, 0
+//   br i1 %cmp5, label %if.then7, label %if.end8
+
+// if.then7:                                         ; preds = %if.end
+//   tail call void @perror(i8* getelementptr inbounds ([37 x i8], [37 x i8]* @.str.5, i64 0, i64 0)) #23
+//   br label %if.end8
+
+// if.end8:                                          ; preds = %if.then7, %if.end
+//   tail call void @free(i8* nonnull %call) #24
+//   tail call void @free(i8* %call1) #24
+//   tail call void @initialize_write(i8* getelementptr inbounds ([16 x i8], [16 x i8]* @IV, i64 0, i64 0), i32 16)
+//   call void @llvm.lifetime.end.p0i8(i64 4, i8* nonnull %0) #24
+//   ret void
+// }
+
+   predicate stateFramingMultiValue(s:state,s':state,ops:set<Data>)
+    {
+        ValidState(s)
+        && ValidState(s')
+        && forall op :: op in ops ==> 
+            (&& ValidData(s,op)
+            && ValidData(s',op)
+            && s.ok == s'.ok
+            && (forall lv :: (lv in s.lvs && !(s.lvs[lv] in ops)) ==> (lv in s'.lvs && s.lvs[lv] == s'.lvs[lv]))//(lv in s'.lv && s.lv[op] == s'.lv[op])
+            && (forall gv :: (gv in s.gvs && !(s.gvs[gv] in ops)) ==> (gv in s'.gvs && s.gvs[gv] == s'.gvs[gv]))
+            && s.m == s'.m)
+    }
+
+    predicate stateFraming(s:state,s':state,op:operand)
+    {
+        ValidState(s)
+        && ValidState(s')
+        && ValidOperand(s,op)
+        && ValidOperand(s',op)
+        && s.ok == s'.ok
+        && op.LV? ==> (forall lv :: (lv in s.lvs && lv != op.l) ==> (lv in s'.lvs && s.lvs[lv] == s'.lvs[lv]))//(lv in s'.lv && s.lv[op] == s'.lv[op])
+        && op.GV? ==> (forall gv :: (gv in s.gvs && gv != op.g) ==> (gv in s'.gvs && s.gvs[gv] == s'.gvs[gv]))//(lv in s'.lv && s.lv[op] == s'.lv[op])
+        && s.m == s'.m
+    }
+
+    predicate MiniSpec(s:LLVM_def.state,cipherText:Data, bytes_written:Data)
+    {
+        && ValidState(s)
+        && forall r:LLVM_def.state :: (evalBlock(encrypt(),s,r) ==> stateFramingMultiValue(s,r,{cipherText,bytes_written})) 
+
+    }
+
+     function encrypt():codes
+        // reads s.m.mem; plainText:Data, s:state
+    {
+        lvm_Codes(Ins(RET(D(Void))),lvm_CNil())    
+    }
+
+    function initialize_write(char_ptr:Data, size:Data):codes
+    {
+        ForeignFunction
+    }
+
+    function free(ptr:Data):codes
+    {
+        ForeignFunction
+    }
+
+    function malloc(ptr:Data):codes
+    {
+        ForeignFunction
+    }
+
+
+    function challenge_prob_5_code_write_encrypted():lvm_code
+    {
+
+       // [temp] dummy ptrs
+        var call := D(Ptr(0,0,0,1));
+        var call1 := (Ptr(0,0,0,1));
+        var IV_SIZE := Int(16,IntType(4,false));
+        var bytes_written := D(Ptr(0,0,0,1));
+ 
+
+        // if.end8:                                          ; preds = %if.then7, %if.end
+        //   tail call void @free(i8* nonnull %call) #24
+        //   tail call void @free(i8* %call1) #24
+        //   tail call void @initialize_write(i8* getelementptr inbounds ([16 x i8], [16 x i8]* @IV, i64 0, i64 0), i32 16)
+        //   call void @llvm.lifetime.end.p0i8(i64 4, i8* nonnull %0) #24
+        //   ret void
+        var if_end8:code := lvm_Block(lvm_Codes(Ins(CALL(D(Void),free(call.d))),
+                                      lvm_Codes(Ins(CALL(D(Void),free(call1))),  
+                                      lvm_Codes(Ins(CALL(D(Void),initialize_write(call1,IV_SIZE))),  
+                                      lvm_Codes(Ins(RET(D(Void))),lvm_CNil()))))); 
+
+        
+        lvm_Block(lvm_Codes(Ins(ALLOCA(bytes_written,4)),
+                  lvm_Codes(Ins(CALL(call,malloc(call.d))),
+                  lvm_Codes(Ins(RET(D(Void))),lvm_CNil()))))                           
+
+    }
+
+
+    //  FULL
+    //   %bytes_written = alloca i32, align 4
+    //   call void @llvm.lifetime.start.p0i8(i64 4, i8* nonnull %0) #24
+    //   %call = tail call noalias align 16 dereferenceable_or_null(112) i8* @malloc(i64 112) #24
+    //   tail call void @llvm.memcpy.p0i8.p0i8.i64(i8* noundef nonnull align 16 dereferenceable(112) %call, i8* noundef nonnull align 8 dereferenceable(112) getelementptr inbounds (%struct.MBlock, %struct.MBlock* @mblock, i64 0, i32 0, i64 0), i64 112, i1 false)
+    //   %call1 = tail call noalias align 16 dereferenceable_or_null(120) i8* @malloc(i64 120) #24
+    //   %call2 = tail call i32 @encrypt(i8* %call, i32 112, i8* getelementptr inbounds ([32 x i8], [32 x i8]* @KEY, i64 0, i64 0), i8* getelementptr inbounds ([16 x i8], [16 x i8]* @IV, i64 0, i64 0), i8* %call1) #24
+    //   store i32 %call2, i32* %bytes_written, align 4, !tbaa !3
+    //   %1 = load %struct._IO_FILE*, %struct._IO_FILE** @wfd, align 8, !tbaa !14
+    //   %call3 = call i64 @fwrite(i8* nonnull %0, i64 4, i64 1, %struct._IO_FILE* %1)
+    //   %cmp = icmp eq i64 %call3, 0
+    //   br i1 %cmp, label %if.then, label %if.end
+
+
+
+}
